refactor

theories/Parallel/ContractEquations.v
@@ -1,6 +1,8 @@
-Require Import CSL.Parallel.Contract CSL.Parallel.TranslationOnly.  
+Require Import CSL.Parallel.Contract.  
 Require Import Lists.List Bool.Bool Bool.Sumbool Setoid Coq.Arith.PeanoNat.
+Require Import micromega.Lia.
 From Equations Require Import Equations.
+Require Import Arith.
 Require Import micromega.Lia.
 (** printing =~ %$=\sim$% *)
 
@@ -163,7 +165,7 @@ Proof.
   intros. auto with eqDB.
 Qed.
 
-
+(********************Soundness*****************************)
 Lemma cons_app : forall (A: Type) (a : A)(l : list A), a::l = [a]++l.
 Proof. auto.
 Qed.
@@ -351,372 +353,6 @@ intros. rewrite (incl_Σ_idemp H).
 rewrite (incl_Σ_idemp H0). apply Σ_app_comm.
 Qed.
 
-
-Equations plus_norm (c : Contract) : (Contract) by  wf (con_size c) :=
-plus_norm  c := if stuck_dec c then Failure
-               else if nu c then Success _+_ Σ (map (fun e => (Event e) _;_ (plus_norm (e \ c))) alphabet)
-                            else             Σ (map (fun e => (Event e) _;_ (plus_norm (e \ c))) alphabet).
-
-Next Obligation. auto using not_stuck_derives. Defined.
-Next Obligation. auto using not_stuck_derives. Defined.
-Global Transparent plus_norm.
-
-
-Lemma plus_norm_cons : forall (e:EventType)(s:Trace)(c:Contract),
-(forall (e : EventType) (s : Trace), s =~ e \ c <-> s =~ plus_norm (e \ c)) ->
-e :: s =~ c <-> e :: s =~ Σ (map (fun e0 : EventType => Event e0 _;_ plus_norm (e0 \ c)) alphabet).
-Proof.
-intros. repeat rewrite derive_spec_comp.
-assert (HA: forall (l : list Contract)(e : EventType), e \ (Σ l) = Σ (map (fun c => e \ c) l)).
-{ intros. induction l. - reflexivity. - simpl. f_equal. assumption. } rewrite HA. rewrite in_Σ.
-rewrite map_map. rewrite H. split;intros.
-- exists (Success _;_ (plus_norm (e \ c))). split.
-  * rewrite in_map_iff. exists e. split;auto with eqDB. 
-    simpl. destruct (EventType_eq_dec e e);[ reflexivity | contradiction ].
-  * rewrite <- (app_nil_l s). constructor; auto with cDB.
-- destruct H0 as [c0 [P0 P1]]. rewrite in_map_iff in P0. destruct P0 as [x [P3 P4]]. subst.
-  simpl in P1. destruct (EventType_eq_dec x e).
-  * inversion P1. inversion H3. subst. simpl. assumption.
-  * inversion P1. inversion H3.
-Qed.
-
-
-Lemma plus_norm_nil : forall (c : Contract), ~([] =~ Σ (map (fun e0 : EventType => Event e0 _;_ plus_norm (e0 \ c)) alphabet)).
-Proof.
-intros. intro H. apply in_Σ in H as [c0 [P0 P1]]. apply in_map_iff in P0 as [e [P P3]]. 
-subst. inversion P1. apply app_eq_nil in H0 as [H0 H00]. subst. inversion H1.
-Qed.
- 
-Theorem plus_norm_spec : forall (c : Contract)(s : Trace), s =~ c <-> s =~ plus_norm c.
-Proof.
-intros. funelim (plus_norm c). destruct (stuck_dec c).
-- apply Stuck_failure. assumption.
-- destruct (nu c) eqn:Heqn.
-  * destruct s.
-    ** split;intros;auto with cDB. auto using Matches_Comp_nil_nu. 
-    ** assert (HA: forall (c : Contract), e::s =~ Success _+_ c <-> e::s =~ c).
-       { split; intros. inversion H0. inversion H3. assumption. auto with cDB. } rewrite HA.
-       apply plus_norm_cons. auto.
-  * destruct s.
-    ** split;intros.
-      *** rewrite Matches_Comp_iff_matchesb in H0. simpl in H0. 
-          rewrite Heqn in H0. discriminate.
-      *** apply plus_norm_nil in H0 as [].
-    ** apply plus_norm_cons. auto.
-Qed.
-
-Lemma Stuck_eq_Failure : forall c, Stuck c -> c =R= Failure.
-Proof.
-intros. induction H;auto with eqDB.
-- rewrite IHStuck1. rewrite IHStuck2. auto_rwd_eqDB.
-- rewrite IHStuck. auto_rwd_eqDB.
-- rewrite IHStuck. rewrite c_par_comm. auto_rwd_eqDB.
-- rewrite IHStuck. auto_rwd_eqDB.
-Qed.
-
-Ltac stuck_tac := 
-   match goal with
-    | [ |- context[if stuck_dec ?c then _ else _ ]] => destruct (stuck_dec c)
-        end.
-
-Lemma plus_norm_Failure : plus_norm Failure =R= Failure.
-Proof.
-simp plus_norm. stuck_tac;auto_rwd_eqDB. inversion n.
-Qed. 
-
-Lemma Σ_Seq_Failure : forall es, Σ (map (fun e : EventType => Event e _;_ plus_norm Failure) es) =R= Failure.
-Proof.
-induction es. simpl. reflexivity.
-simpl. rewrite IHes. auto_rwd_eqDB.
-Qed.
-
-Lemma plus_norm_Success : plus_norm Success =R= Success.
-Proof.
-simp plus_norm. stuck_tac. symmetry. auto using Stuck_eq_Failure.
-simpl. rewrite Σ_Seq_Failure. auto_rwd_eqDB.
-Qed. 
-
-Hint Rewrite plus_norm_Failure plus_norm_Success : eqDB.
-
-Lemma map_ext_in_R :
-  forall (A : Type)(f g:A->Contract) l, (forall a, In a l -> f a =R= g a) -> Σ (map f l) =R= Σ (map g l).
-Proof.
-induction l;intros;simpl;auto with eqDB.
-apply c_plus_ctx. apply H. apply in_eq. apply IHl.
-intros. apply H. simpl. now right.
-Qed.
-
-(*
-Lemma ext_in_map_R :
-  forall (A : Type)(f g:A->Contract) l, Σ (map f l) =R= Σ (map g l) -> forall a, In a l -> f a =R= g a.
-Proof.
-induction l;intros. simpl in H0. contradiction.
-simpl in H0. destruct H0.
-- subst. simpl in H. apply IHl. apply map_ext_in_R.
-*)
-
-Inductive Atom : Contract -> Prop :=
-| AFailure : Atom Failure
-| ASuccess : Atom Success.
-
-Inductive NormalForm : Contract -> Prop :=
-| NFF: NormalForm Failure
-| NFS: NormalForm Success
-| NFList es l (H1: forall a, In a l -> NormalForm a) : NormalForm (Σ (map (fun x => Event (fst x) _;_ snd x) (combine es l)))
-| NFListS es l  (H1: forall a, In a l -> NormalForm a) : NormalForm (Success _+_ Σ (map (fun x => Event (fst x) _;_ snd x) (combine es l))).
-
-Lemma Sequential_Σ : forall l, Forall Sequential l -> Sequential (Σ l).
-Proof.
-induction l;intros.
-- simpl. constructor.
-- simpl. rewrite Forall_forall in H. constructor.
-  apply H. apply in_eq. apply IHl. rewrite <- Forall_forall in H.
-  inversion H. auto.
-Qed.
-
-
-Lemma NormalForm_i_Sequential : forall c, NormalForm c -> Sequential c.
-Proof.
-intros. induction H;auto with eqDB.
-- apply Sequential_Σ. rewrite Forall_forall in *. intros.
-  rewrite in_map_iff in H0. destruct_ctx. subst. constructor.
-  constructor. destruct x0. apply in_combine_r in H2. auto.
-- constructor;auto with eqDB. apply Sequential_Σ. rewrite Forall_forall in *. intros.
-  rewrite in_map_iff in H0. destruct_ctx. subst. constructor.
-  constructor. destruct x0. apply in_combine_r in H2. auto.
-Qed.
-
-Lemma NormalForm_trans : forall c, NormalForm c -> exists c', translate_aux c = Some c'.
-Proof.
-intros. apply translate_aux_sequential. auto using NormalForm_i_Sequential.
-Qed.
-
-
-Lemma Σ_extend : forall l c, c _+_ Σ l = Σ (c :: l ).
-Proof.
-induction l;intros. auto. simpl. auto.
-Qed.
-
-Lemma decompose_map : 
-forall es c, map (fun e => Event e _;_ plus_norm (e \ c)) es = map (fun x => (Event (fst x) _;_ snd x)) (combine es (map (fun e => plus_norm (e \ c) ) es)).
-Proof.
-induction es;intros.
-- simpl. auto.
-- simpl. rewrite IHes. auto.
-Qed. 
-
-Lemma plus_norm_NormalForm : forall c, NormalForm (plus_norm c).
-Proof.
-intros. funelim (plus_norm c). stuck_tac.
-- constructor.
-- destruct (nu c).
-  * rewrite decompose_map. erewrite map_ext. eapply NFListS.
-    intros. rewrite in_map_iff in H0. destruct_ctx.
-    subst. auto. intros. destruct a. simpl. auto.
-  * rewrite decompose_map. erewrite map_ext. eapply NFList.
-    intros. rewrite in_map_iff in H0. destruct_ctx.
-    subst. auto. intros. destruct a. simpl. auto.
-Qed.
-
-Lemma plus_norm_trans : forall c, exists c', translate_aux (plus_norm c) = Some c'.
-Proof.
-intros. eauto using plus_norm_NormalForm, NormalForm_trans.
-Qed.
-(*
-Lemma plus_norm_core : forall c0 c1 c0' c1', tra c0 = Some c0' -> translate c1 = Some c1'
--> (forall s, s=~ c0 <-> s =~ c1 ) -> c0' =R= c1'.*)
-(*
-Lemma NormalFormEvent : forall l e , 
-NormalForm (Σ (map (fun e0 => Event e0 _;_ plus_norm (if EventType_eq_dec e e0 then Success else Failure)) l)).
-Proof.
-intros.
-induction l;intros.
-- simpl. constructor. constructor.
-- simpl. eq_event_destruct;subst.
-  * rewrite Σ_extend. constructor. rewr con*)
-
-(*
-Lemma Σ_Seq_Event : forall alphabet0 e, (forall e', In e' alphabet0) ->
-Σ
-  (map (fun e0 : EventType => Event e0 _;_ plus_norm (if EventType_eq_dec e e0 then Success else Failure))
-     alphabet0) =R= Event e.
-Proof. intros.
-eapply c_core;simpl;eauto. destruct e. simpl.
-induction alphabet0;intros.
-- simpl in H. contradiction.
-- simpl. rewrite IHalphabet0.
-intros.*)
-(*
-Fixpoint translate_aux_core c :=
-match c with
-| CSLC.Failure => CSLC.Failure
-| CSLC.Event e => CSLEQ.Σ (map (fun e1 => CSLC.CSeq (CSLC.Event e1) (CSLC.derive e)(if EventType_eq_dec e e1 then CSLC.Success else CSLC.Failure)) alphabet0)).
-
-Lemma translate_aux_Event : forall alphabet0 e x, 
-translate_aux (Σ (map (fun e0 : EventType => Event e0 _;_ plus_norm (if EventType_eq_dec e e0 then Success else Failure)) alphabet0)) =
-Some x -> CSLEQ.c_eq x
-(CSLEQ.Σ (map (fun e1 => CSLC.CSeq (CSLC.Event e1) (if EventType_eq_dec e e1 then CSLC.Success else CSLC.Failure)) alphabet0)).
-Proof.
-induction alphabet0;intros. 
-- simpl in*. inversion H;subst. constructor.
-- simpl. eq_event_destruct;subst.
-  * rewrite IHalphabet0. simpl. auto.
-intros.
-    Some x
-
-Lemma trans_plus_norm_Event : forall e x, translate_aux (plus_norm (Event e)) = Some x -> CSLEQ.c_eq (CSLC.Event e) x.
-Proof. 
-intros. simp plus_norm in H. simpl in H.*)
-
-Lemma derive_Success : forall e, e \ Success = Failure.
-Proof.
-intros. destruct e;auto.
-Qed.
-(*
-Lemma Σ_event : forall l e c, (forall c', In c' (c::l) -> c =R= Failure \/ c =R= Event e) -> Σ (c::l) =R= Event e.
-Proof.
-induction l;intros.
-simpl. auto_rwd_eqDB. specialize 
-now right.
-simpl. left. specialize IHl with e. simpl in H.
-specialize H with a.
--
-simpl.
-
-*)
-
-Lemma Σ_event : forall l e,
-Σ (map (fun a => Event e _;_ (if EventType_eq_dec e a then Success else Failure)) l) =R= 
-Event e _;_  Σ (map (fun a => (if EventType_eq_dec e a then Success else Failure)) l).
-Proof.
-induction l;intros.
-- simpl. auto_rwd_eqDB.
-- simpl. rewrite IHl. auto_rwd_eqDB.
-Qed.
-
-Lemma or_imp : forall (A B C : Prop), (A \/ B -> C) -> (A -> C) /\ (B -> C). 
-Proof.
-intros. split;auto.
-Qed.
-(*
-Lemma Σ_Success : forall l, (exists c, In c l /\ c =R= Success) -> (forall c, In c l -> c =R= Success \/ c =R= Failure) -> Σ l =R= Success.
-Proof.
-induction l;intros.
-- destruct_ctx. simpl in H. contradiction.
-- destruct_ctx. simpl in *. destruct H.
-  subst.
-  * rewrite H1. rewrite IHl.
-  * specialize H0 with a. apply or_imp in H0. destruct H0.
-    destruct H0;auto. rewrite H0. auto_rwd_eqDB.
-    rewrite H0. auto_rwd_eqDB.
-  *
-
-destruct H;subst.
-    ** rewrite H1. auto_rwd_eqDB.
-    ** specialize H0 with a. apply or_imp in H0. destruct H0.
-       destruct H0;auto. rewrite H0.
-  * destruct H;s ubst.
-    ** rewrite H1. 
-  rewrite IHl. auto_rwd_eqDB.  subst. simpl.*)
-
-
-Lemma Σ_alphabet_or : forall alphabet0 e ,
- Σ (map (fun a : CSLC.EventType => if EventType_eq_dec e a then Success else Failure) alphabet0) =R= Success /\ In e alphabet0 \/
- Σ (map (fun a : CSLC.EventType => if EventType_eq_dec e a then Success else Failure) alphabet0) =R= Failure /\ ~(In e alphabet0).
-Proof.
-induction alphabet0;intros.
-- simpl. now right.
-- simpl. eq_event_destruct.
-  * subst. edestruct IHalphabet0.
-    ** destruct H. left. split.
-       rewrite H. auto_rwd_eqDB. now left.
-    ** destruct H. rewrite H.
-       auto_rwd_eqDB.
-  * edestruct IHalphabet0.
-    ** destruct H. rewrite H. auto_rwd_eqDB.
-    ** destruct H. rewrite H. auto_rwd_eqDB.
-       right. split;auto with eqDB. intro H2. destruct H2.
-       symmetry in H1. contradiction. contradiction.
-Qed.
-
-Lemma Σ_alphabet : forall e, Σ (map (fun a => if EventType_eq_dec e a then Success else Failure) alphabet) =R= Success.
-Proof.
-intros. destruct (Σ_alphabet_or alphabet e).
-- destruct H. auto.
-- destruct H. pose proof (in_alphabet e). contradiction.
-Qed.
-
-Lemma Σ_decompose_fun : forall (A: Type) l (P P' : A -> Contract),
-Σ (map (fun a : A => P a _+_ P' a) l) =R= Σ (map (fun a : A => P a) l) _+_  Σ (map (fun a : A => P' a) l).
-Proof.
-induction l;intros.
-- simpl. auto_rwd_eqDB.
-- simpl. rewrite c_plus_assoc. rewrite c_plus_assoc. apply c_plus_ctx;auto with eqDB.
-  rewrite (c_plus_comm (Σ _)).
-  rewrite c_plus_assoc. apply c_plus_ctx;auto with eqDB. rewrite IHl.
-  auto_rwd_eqDB.
-Qed.
-
-Lemma Σ_decompose_Seq : forall l (P: EventType -> Contract) c,
-Σ (map (fun a  => P a _;_ c) l) =R= Σ (map (fun a  => P a) l) _;_ c.
-Proof.
-induction l;intros.
-- simpl. auto_rwd_eqDB.
-- simpl. auto_rwd_eqDB.
-Qed.
-
-Lemma Σ_decompose_Seq_l : forall l (P: EventType -> Contract) c,
-Σ (map (fun a  => c _;_ P a) l) =R= c _;_ Σ (map (fun a  => P a) l).
-Proof.
-induction l;intros.
-- simpl. auto_rwd_eqDB.
-- simpl. auto_rwd_eqDB.
-Qed.
-
-
-Lemma Σ_par_distr_aux : forall l1 c (P' : EventType -> Contract),
-c _*_ Σ (map (fun a0 : EventType => P' a0) l1) =R=
-Σ (map (fun a' : EventType => c _*_ P' a') l1).
-Proof.
-induction l1;intros.
-- simpl. auto_rwd_eqDB.
-- simpl. rewrite <- IHl1. auto_rwd_eqDB.
-Qed.
-
-Lemma Σ_par_distr : forall l0 l1 (P P' : EventType -> Contract),
-Σ (map (fun a  => P a) l0) _*_ Σ (map (fun a => P' a) l1) =R=
-Σ (map (fun aa  => P (fst aa) _*_ P' (snd aa)) (list_prod l0 l1)).
-Proof. 
-induction l0;intros.
-- simpl. auto_rwd_eqDB.
-- simpl.  auto_rwd_eqDB.
-  rewrite map_app. rewrite Σ_app. apply c_plus_ctx.
-  * rewrite map_map. simpl. apply Σ_par_distr_aux.
-  * auto_rwd_eqDB.
-Qed. 
-
-
-Lemma Σ_par_distr_aux_r : forall l1 c (P' : EventType -> Contract),
-Σ (map (fun a0 : EventType => P' a0) l1) _*_ c =R=
-Σ (map (fun a' : EventType => P' a' _*_ c) l1).
-Proof.
-induction l1;intros.
-- simpl. auto_rwd_eqDB.
-- simpl. rewrite <- IHl1. auto_rwd_eqDB.
-Qed.
-(*
-Lemma Σ_par_distr_r : forall l0 l1 (P P' : EventType -> Contract),
-Σ (map (fun a  => P a) l0) _*_ Σ (map (fun a => P' a) l1) =R=
-Σ (map (fun aa  => P (fst aa) _*_ P' (snd aa)) (list_prod l0 l1)).
-Proof. 
-induction l0;intros.
-- simpl. auto_rwd_eqDB.
-- simpl.  auto_rwd_eqDB.
-  rewrite map_app. rewrite Σ_app. apply c_plus_ctx.
-  * rewrite map_map. simpl. apply Σ_par_distr_aux.
-  * auto_rwd_eqDB.
-Qed. *)
-
 Definition o c := if nu c then Success else Failure.
 
 Lemma o_plus : forall c0 c1, o (c0 _+_ c1) =R= o c0 _+_ o c1.
@@ -754,73 +390,403 @@ Hint Rewrite o_plus o_seq o_par : eqDB.
 
 Hint Rewrite o_true o_false : oDB.
 
+
+(******************Translation***************)
+
+Inductive Stuck : Contract -> Prop :=
+ | STFailure : Stuck Failure
+ | STPLus c0 c1 (H0 : Stuck c0) (H1 : Stuck c1) : Stuck (c0 _+_ c1)
+ | STSeq c0 c1 (H0 : Stuck c0) : Stuck (c0 _;_ c1)
+ | STParL c0 c1 (H0 : Stuck c0) : Stuck (c0 _*_ c1)
+ | STParR c0 c1 (H1 : Stuck c1) : Stuck (c0 _*_ c1).
+Hint Constructors Stuck : tDB.
+
+Inductive NotStuck : Contract -> Prop :=
+ | NSTSuccess : NotStuck Success
+ | NSEvent e : NotStuck (Event e)
+ | NSTPlusL c0 c1 (H0 : NotStuck c0) : NotStuck (c0 _+_ c1)
+ | NSTPlusR c0 c1 (H1 : NotStuck c1) : NotStuck (c0 _+_ c1)
+ | NSTSeq c0 c1 (H0 : NotStuck c0) : NotStuck (c0 _;_ c1)
+ | NSTPar c0 c1 (H0 : NotStuck c0)(H1 : NotStuck c1) : NotStuck (c0 _*_ c1).
+
+Hint Constructors NotStuck : tDB.
+
+Fixpoint stuck (c : Contract) :=
+match c with
+| Failure => true
+| c0 _+_ c1 => stuck c0 && stuck c1
+| c0 _;_ _ => stuck c0
+| c0 _*_ c1 => stuck c0 || stuck c1
+| _ => false
+end.
+
+
+
+Lemma stuck_false : forall (c : Contract), stuck c = false -> NotStuck c.
+Proof.
+induction c; intros;simpl in*;auto with tDB bool; try discriminate.
+apply andb_false_elim in H as [H | H]; auto with tDB.
+apply orb_false_iff in H as [H1 H2]; auto with tDB.
+Defined.
+
+Lemma stuck_true : forall (c : Contract), stuck c = true -> (Stuck c).
+Proof.
+induction c; intros; simpl in *; auto with tDB; try discriminate. 
+apply orb_prop in H as [H | H]; auto with tDB.
+Defined.
+
+
+Definition stuck_dec (c : Contract) : {Stuck c}+{NotStuck c}.
+Proof. destruct (stuck c) eqn:Heqn; auto using stuck_true || auto using stuck_false.
+Defined.
+
+Lemma NotStuck_negation : forall (c : Contract), NotStuck c -> ~(Stuck c).
+Proof.
+intros. induction H ; intro H2; inversion H2.
+all : inversion H2; contradiction.
+Qed.
+
+Fixpoint con_size (c:Contract):nat :=
+match c with
+| Failure => 0
+| Success => 1
+| Event _ => 2
+| c0 _+_ c1 => max (con_size c0) (con_size c1) 
+| c0 _;_ c1 => if stuck_dec c0 then 0 else (con_size c0) + (con_size c1)
+| c0 _*_ c1 => if  sumbool_or _ _ _ _ (stuck_dec c0) (stuck_dec c1) then 0 else (con_size c0) + (con_size c1)
+end.
+
+Ltac stuck_tac :=
+  (repeat match goal with
+         | [ H : _ /\ _ |- _ ] => destruct H
+         | [ |- context[if ?a then _ else _] ] => destruct a
+         | [ H: Stuck ?c0, H1: NotStuck ?c0  |- _ ] => apply NotStuck_negation in H1; contradiction
+  end);auto with tDB.
+
+
+
+Lemma stuck_0 : forall (c : Contract), Stuck c -> con_size c = 0.
+Proof.
+intros. induction H;auto;simpl; try solve [ lia | stuck_tac].
+Defined.
+
+Lemma stuck_not_nullary : forall (c : Contract), Stuck c -> nu c = false.
+Proof.
+intros. induction H; simpl ;subst ;auto with bool.
+all : rewrite IHStuck. all: auto with bool.
+rewrite andb_comm. auto with bool.
+Defined.
+
+Lemma Stuck_derive : forall (c : Contract)(e : EventType), Stuck c -> Stuck (e \ c).
+Proof.
+intros. induction H; simpl in *.
+- constructor.
+- constructor; auto.
+- apply stuck_not_nullary in H. rewrite H. auto with tDB.
+- auto with tDB.
+- auto with tDB.
+Qed.
+
+
+
+Lemma Stuck_derive_0 : forall (c : Contract)(e:EventType), Stuck c -> con_size (e \ c) = 0.
+Proof.
+intros. apply stuck_0. apply Stuck_derive. assumption.
+Qed.
+
+Ltac NotStuck_con H := apply NotStuck_negation in H; contradiction.
+
+Lemma NotStuck_0lt : forall (c : Contract), NotStuck c -> 0 < con_size c.
+Proof.
+intros. induction H; simpl ; try lia.
+- stuck_tac. lia.
+- stuck_tac. destruct o0; stuck_tac. lia.
+Defined.
+
+
+Lemma not_stuck_derives : forall (c : Contract), NotStuck c -> (forall (e : EventType), con_size (e \ c) < con_size c).
+Proof.
+intros. induction c.
+- simpl. lia.
+- inversion H.
+- simpl. destruct (EventType_eq_dec e0 e) ; simpl ; lia.
+- simpl. inversion H.
+  * destruct (stuck_dec c2).
+    ** apply stuck_0 in s as s2. rewrite (Stuck_derive_0 _ s). rewrite Max.max_comm. simpl. 
+       apply Max.max_case_strong.
+      *** intros. auto.
+      *** intros. rewrite s2 in H3. pose proof (NotStuck_0lt H1). lia.
+    ** apply IHc1 in H1. apply IHc2 in n. lia.
+  * destruct (stuck_dec c1).
+    ** apply stuck_0 in s as s2. rewrite (Stuck_derive_0 _ s). simpl. 
+       apply Max.max_case_strong.
+      *** intros. rewrite s2 in H3. pose proof (NotStuck_0lt H0). lia.
+      *** intros. auto.
+    ** apply IHc1 in n. apply IHc2 in H0. lia.
+- inversion H. subst. simpl. destruct (nu c1) eqn:Heqn.
+  * destruct (stuck_dec c1). apply NotStuck_negation in H1. contradiction.
+    simpl. destruct (stuck_dec (e \ c1)).
+    ** simpl. destruct (stuck_dec c2).
+      *** rewrite Stuck_derive_0. pose proof (NotStuck_0lt H1). lia. assumption.
+      *** rewrite <- (plus_O_n (con_size (e \ c2))). apply IHc2 in n0. lia.
+    ** apply IHc1 in H1. destruct (stuck_dec c2).
+
+      *** rewrite (Stuck_derive_0 _ s). rewrite Max.max_comm.  simpl.  apply plus_lt_compat_r.  assumption. 
+      *** apply IHc1 in n. apply IHc2 in n1. lia.
+  * destruct (stuck_dec c1).
+    ** apply NotStuck_negation in H1. contradiction.
+    ** simpl. destruct (stuck_dec (e \ c1)).
+      *** pose proof (NotStuck_0lt H1). lia.
+      *** apply Plus.plus_lt_compat_r. auto.
+- inversion H. subst. simpl. destruct (sumbool_or (Stuck (e \ c1)) (NotStuck (e \ c1))
+                                      (Stuck c2) (NotStuck c2) (stuck_dec (e \ c1))
+      (                                 stuck_dec c2)) as [[o | o] | o].
+  * destruct (sumbool_or (Stuck c1) (NotStuck c1) 
+      (Stuck (e \ c2)) (NotStuck (e \ c2)) 
+      (stuck_dec c1) (stuck_dec (e \ c2))) as [[o0 | o0] | o0].
+    ** NotStuck_con H2.
+    ** simpl. destruct (sumbool_or (Stuck c1) (NotStuck c1) (Stuck c2)
+    (NotStuck c2) (stuck_dec c1) (stuck_dec c2)) as [[o1 | o1] | o1].
+      *** NotStuck_con H2.
+      *** NotStuck_con H3.
+      *** pose proof (NotStuck_0lt H2). lia.
+    ** destruct (sumbool_or (Stuck c1) (NotStuck c1) (Stuck c2)
+    (NotStuck c2) (stuck_dec c1) (stuck_dec c2)) as [[o1 | o1] | o1].
+      *** NotStuck_con H2. 
+      *** NotStuck_con H3. 
+      *** simpl. apply plus_lt_compat_l. auto. 
+  * NotStuck_con H3. 
+  * destruct o. destruct (sumbool_or (Stuck c1) (NotStuck c1) 
+      (Stuck (e \ c2)) (NotStuck (e \ c2)) 
+      (stuck_dec c1) (stuck_dec (e \ c2))) as [[o0 | o0] | o0].
+    ** NotStuck_con H2. 
+    ** destruct (sumbool_or (Stuck c1) (NotStuck c1) (Stuck c2)
+    (NotStuck c2) (stuck_dec c1) (stuck_dec c2)) as [[o | o] | o].
+      *** NotStuck_con H2.
+      *** NotStuck_con H3.
+      *** rewrite Max.max_comm. simpl. apply plus_lt_compat_r. auto.
+    ** destruct (sumbool_or (Stuck c1) (NotStuck c1) (Stuck c2)
+    (NotStuck c2) (stuck_dec c1) (stuck_dec c2)) as [[o | o] | o].
+      *** NotStuck_con H2.
+      *** NotStuck_con H3.
+      *** apply Max.max_case_strong. 
+        **** intros. apply plus_lt_compat_r. auto.
+        **** intros. apply plus_lt_compat_l. auto.
+Qed.
+
+Lemma Stuck_failure : forall (c : Contract), Stuck c -> (forall s, s =~ c <-> s =~ Failure).
+Proof.
+intros. split. 2: { intros. inversion H0. }
+generalize dependent s.  induction c; intros.
+- inversion H.
+- assumption. 
+- inversion H.
+- inversion H. inversion H0; auto.
+- inversion H. inversion H0. apply IHc1 in H7. inversion H7. assumption.
+- inversion H0. inversion H.
+  * eapply IHc1 in H8. inversion H8. eauto.
+  * eapply IHc2 in H8. inversion H8. eauto.
+Qed.
+
+
+Equations plus_norm (c : Contract) : (Contract) by  wf (con_size c) :=
+plus_norm  c := if stuck_dec c then Failure
+               else (o c) _+_ Σ (map (fun e => (Event e) _;_ (plus_norm (e \ c))) alphabet).
+
+Next Obligation. auto using not_stuck_derives. Defined.
+
+(*Global Transparent plus_norm.*)
+
+
+Lemma plus_norm_cons : forall (e:EventType)(s:Trace)(c:Contract),
+(forall (e : EventType) (s : Trace), s =~ e \ c <-> s =~ plus_norm (e \ c)) ->
+e :: s =~ c <-> e :: s =~ Σ (map (fun e0 : EventType => Event e0 _;_ plus_norm (e0 \ c)) alphabet).
+Proof.
+intros. repeat rewrite derive_spec_comp.
+assert (HA: forall (l : list Contract)(e : EventType), e \ (Σ l) = Σ (map (fun c => e \ c) l)).
+{ intros. induction l. - reflexivity. - simpl. f_equal. assumption. } rewrite HA. rewrite in_Σ.
+rewrite map_map. rewrite H. split;intros.
+- exists (Success _;_ (plus_norm (e \ c))). split.
+  * rewrite in_map_iff. exists e. split;auto with eqDB. 
+    simpl. destruct (EventType_eq_dec e e);[ reflexivity | contradiction ].
+  * rewrite <- (app_nil_l s). constructor; auto with cDB.
+- destruct H0 as [c0 [P0 P1]]. rewrite in_map_iff in P0. destruct P0 as [x [P3 P4]]. subst.
+  simpl in P1. destruct (EventType_eq_dec x e).
+  * inversion P1. inversion H3. subst. simpl. assumption.
+  * inversion P1. inversion H3.
+Qed.
+
+
+Lemma plus_norm_nil : forall (c : Contract), ~([] =~ Σ (map (fun e0 : EventType => Event e0 _;_ plus_norm (e0 \ c)) alphabet)).
+Proof.
+intros. intro H. apply in_Σ in H as [c0 [P0 P1]]. apply in_map_iff in P0 as [e [P P3]]. 
+subst. inversion P1. apply app_eq_nil in H0 as [H0 H00]. subst. inversion H1.
+Qed.
+ 
+Theorem plus_norm_spec : forall (c : Contract)(s : Trace), s =~ c <-> s =~ plus_norm c.
+Proof.
+intros. funelim (plus_norm c). destruct (stuck_dec c).
+- apply Stuck_failure. assumption.
+- unfold o. destruct (nu c) eqn:Heqn.
+  * destruct s.
+    ** split;intros;auto with cDB. auto using Matches_Comp_nil_nu. 
+    ** assert (HA: forall (c : Contract), e::s =~ Success _+_ c <-> e::s =~ c).
+       { split; intros. inversion H0. inversion H3. assumption. auto with cDB. } rewrite HA.
+       apply plus_norm_cons. auto.
+  * destruct s.
+    ** split;intros.
+      *** rewrite Matches_Comp_iff_matchesb in H0. simpl in H0. 
+          rewrite Heqn in H0. discriminate.
+      *** c_inversion. apply plus_norm_nil in H3 as [].
+    ** split;intros. apply MPlusR. rewrite <- plus_norm_cons;auto.
+       c_inversion. rewrite plus_norm_cons;auto. 
+Qed.
+
+(**********plus_norm respects axiomatization *******)
+
+
+
+Lemma Stuck_eq_Failure : forall c, Stuck c -> c =R= Failure.
+Proof.
+intros. induction H;auto with eqDB.
+- rewrite IHStuck1. rewrite IHStuck2. auto_rwd_eqDB.
+- rewrite IHStuck. auto_rwd_eqDB.
+- rewrite IHStuck. rewrite c_par_comm. auto_rwd_eqDB.
+- rewrite IHStuck. auto_rwd_eqDB.
+Qed.
+
+
+
+Lemma plus_norm_Failure : plus_norm Failure =R= Failure.
+Proof.
+simp plus_norm. stuck_tac;auto_rwd_eqDB. inversion n.
+Qed. 
+
+Lemma Σ_Seq_Failure : forall es, Σ (map (fun e : EventType => Event e _;_ plus_norm Failure) es) =R= Failure.
+Proof.
+induction es. simpl. reflexivity.
+simpl. rewrite IHes. auto_rwd_eqDB.
+Qed.
+
+Lemma plus_norm_Success : plus_norm Success =R= Success.
+Proof.
+simp plus_norm. stuck_tac. symmetry. auto using Stuck_eq_Failure.
+simpl. rewrite Σ_Seq_Failure. auto_rwd_eqDB.
+Qed. 
+
+Hint Rewrite plus_norm_Failure plus_norm_Success : eqDB.
+
+Lemma map_ext_in_R :
+  forall (A : Type)(f g:A->Contract) l, (forall a, In a l -> f a =R= g a) -> Σ (map f l) =R= Σ (map g l).
+Proof.
+induction l;intros;simpl;auto with eqDB.
+apply c_plus_ctx. apply H. apply in_eq. apply IHl.
+intros. apply H. simpl. now right.
+Qed.
+
+
+
+
+
 Ltac eq_m_left := repeat rewrite c_plus_assoc; apply c_plus_ctx;
                   auto_rwd_eqDB.
 
 Ltac eq_m_right := repeat rewrite <- c_plus_assoc; apply c_plus_ctx;
                   auto_rwd_eqDB.
-(*
-Lemma derive_eq : forall e c,
-o c _+_ Event e _;_ e \ c =R= c  \/
-e \ c =R= Failure.
-Proof.
-induction c;intros;simpl.
-- left. auto_rwd_eqDB. 
-- left. auto_rwd_eqDB.
-- eq_event_destruct;auto_rwd_eqDB. subst. now left.
-- destruct IHc1; destruct IHc2.
-  * rewrite <- H at 3. rewrite <- H0 at 3. left.
-    auto_rwd_eqDB. rewrite (c_plus_assoc _ (_ _;_ _)).
-    rewrite (c_plus_comm (_ _;_ _) (o c2 _+_ _)).
-    eq_m_left.
-  * rewrite H0. auto_rwd_eqDB. left. rewrite c_plus_assoc. 
-    rewrite (c_plus_comm _ (_ _;_ _)). rewrite <- c_plus_assoc.
-    rewrite H. (o _)). 
 
-    
-    destruct (nu c1). simpl. 
-    ** destruct (nu c2).
-      *** auto_rwd_eqDB. rewrite c_plus_assoc. rewrite (c_plus_comm _ (Success _+_ _)).
-          repeat rewrite <- (c_plus_assoc). rewrite c_plus_idemp.
-          repeat rewrite c_plus_assoc.  
-          apply c_plus_ctx. reflexivity. auto_rwd_eqDB.
-      *** auto_rwd_eqDB.
-    ** simpl. destruct (nu c2).
-      *** auto_rwd_eqDB. rewrite c_plus_comm.
-          repeat rewrite c_plus_assoc. apply c_plus_ctx.
-          reflexivity. auto_rwd_eqDB.
-      *** auto_rwd_eqDB.
-  *
- _ Success) .
-          rewrite c_plus_comm. specialize IHc1 with e. destruct IHc1.
-  * left. setoid_rewrite <- H at 3. destruct_ctx. setoid_rewrite H0 at 1. 
-  setoid_rewrite H at 1.*)
-(*
-Lemma test : forall alphabet0 c1 c2,
-Σ (map (fun a : EventType => Event a _;_ (a \ c1 _*_ c2)) alphabet0) _+_ Σ (map (fun a : EventType => Event a _;_ (c1 _*_ a \ c2)) alphabet0) =R=
-o c1 _*_ (Σ (map (fun a : EventType => Event a _;_ a \ c2) alphabet0) _+_
-o c2 _*_ Σ (map (fun a : EventType => Event a _;_ a \ c1) alphabet0) _+_
-Σ (map (fun a : EventType => Event a _;_ a \ c1) alphabet0)) _*_ Σ (map (fun a : EventType => Event a _;_ a \ c2) alphabet0) .
+
+
+Lemma Σ_alphabet_or : forall alphabet0 e ,
+ Σ (map (fun a : CSLC.EventType => if EventType_eq_dec e a then Success else Failure) alphabet0) =R= Success /\ In e alphabet0 \/
+ Σ (map (fun a : CSLC.EventType => if EventType_eq_dec e a then Success else Failure) alphabet0) =R= Failure /\ ~(In e alphabet0).
 Proof.
 induction alphabet0;intros.
-- simpl. auto_rwd_eqDB.
-- simpl. rewrite (c_plus_comm (Event a _;_ (c1 _*_ a \ c2))).
-  repeat rewrite <- (c_plus_assoc _ (Σ _)) .
-  rewrite (c_plus_assoc (_ _;_ _)). rewrite IHalphabet0.
-  destruct (o_destruct c1); rewrite H in *.
-  * destruct (o_destruct c2); rewrite H0 in *.
-    ** repeat rewrite (c_par_neut_l).
+- simpl. now right.
+- simpl. eq_event_destruct.
+  * subst. edestruct IHalphabet0.
+    ** destruct H. left. split.
+       rewrite H. auto_rwd_eqDB. now left.
+    ** destruct H. rewrite H.
        auto_rwd_eqDB.
-       rewrite (c_par_comm (_ _+_ _)).
-       auto_rwd_eqDB. 
-       rewrite (c_plus_comm ((Σ _) _*_ (Σ _))).
-       rewrite <- (c_plus_comm (_ _;_ (c1 _*_ a \ c2))).
-Check c_par_event.
-       rewrite <- c_plus_assoc.
+  * edestruct IHalphabet0; destruct H; rewrite H; auto_rwd_eqDB.
+    right. split;auto with eqDB. intro H2. destruct H2.
+    symmetry in H1. contradiction. contradiction.
+Qed.
 
-    autorewrite with eqDB in *.
-    **
-   in H. rewrite IHalphabet0.*)
+(************Summation rules *****)
+Lemma Σ_alphabet : forall e, Σ (map (fun a => if EventType_eq_dec e a then Success else Failure) alphabet) =R= Success.
+Proof.
+intros. destruct (Σ_alphabet_or alphabet e).
+- destruct H. auto.
+- destruct H. pose proof (in_alphabet e). contradiction.
+Qed.
+
+Lemma Σ_split_plus : forall (A: Type) l (P P' : A -> Contract),
+Σ (map (fun a : A => P a _+_ P' a) l) =R= Σ (map (fun a : A => P a) l) _+_  Σ (map (fun a : A => P' a) l).
+Proof.
+induction l;intros.
+- simpl. auto_rwd_eqDB.
+- simpl. rewrite c_plus_assoc. rewrite c_plus_assoc. apply c_plus_ctx;auto with eqDB.
+  rewrite (c_plus_comm (Σ _)).
+  rewrite c_plus_assoc. apply c_plus_ctx;auto with eqDB. rewrite IHl.
+  auto_rwd_eqDB.
+Qed.
+
+Lemma Σ_factor_seq_r : forall l (P: EventType -> Contract) c,
+Σ (map (fun a  => P a _;_ c) l) =R= Σ (map (fun a  => P a) l) _;_ c.
+Proof.
+induction l;intros.
+- simpl. auto_rwd_eqDB.
+- simpl. auto_rwd_eqDB.
+Qed.
+
+Lemma Σ_factor_seq_l : forall l (P: EventType -> Contract) c,
+Σ (map (fun a  => c _;_ P a) l) =R= c _;_ Σ (map (fun a  => P a) l).
+Proof.
+induction l;intros.
+- simpl. auto_rwd_eqDB.
+- simpl. auto_rwd_eqDB.
+Qed.
+
+
+Lemma Σ_factor_par_l : forall l1 c (P' : EventType -> Contract),
+Σ (map (fun a' : EventType => c _*_ P' a') l1) =R=
+c _*_ Σ (map (fun a0 : EventType => P' a0) l1).
+Proof.
+induction l1;intros.
+- simpl. auto_rwd_eqDB.
+- simpl. rewrite IHl1. auto_rwd_eqDB.
+Qed.
+
+Lemma Σ_factor_par_r : forall l1 c (P' : EventType -> Contract),
+Σ (map (fun a0 : EventType => P' a0) l1) _*_ c =R=
+Σ (map (fun a' : EventType => P' a' _*_ c) l1).
+Proof.
+induction l1;intros.
+- simpl. auto_rwd_eqDB.
+- simpl. rewrite <- IHl1. auto_rwd_eqDB.
+Qed.
+
+Lemma Σ_par_ΣΣ : forall l0 l1 (P0 P1 : EventType -> Contract),
+Σ (map (fun a0  => P0 a0) l0) _*_ Σ (map (fun a1 => P1 a1) l1) =R=
+Σ (map (fun a0  => Σ (map (fun a1  => (P0 a0) _*_ (P1 a1)) l1)) l0).
+Proof. 
+induction l0;intros.
+- simpl. auto_rwd_eqDB.
+- simpl. auto_rwd_eqDB.
+  rewrite Σ_factor_par_l. rewrite IHl0.  reflexivity. 
+Qed. 
+
+
+Lemma ΣΣ_prod_swap : forall l0 l1 (P : EventType -> EventType -> Contract), 
+Σ (map (fun a0 => Σ (map (fun a1 => P a0 a1) l1)) l0)=R=
+Σ (map (fun a0 => Σ (map (fun a1 => P a1 a0) l0)) l1).
+Proof.
+induction l0;intros.
+- simpl. induction l1;intros;simpl;auto with eqDB. rewrite IHl1.
+  auto with eqDB.
+- simpl. rewrite Σ_split_plus. eq_m_left.
+Qed.
 
 Lemma fold_Failure : forall l, Σ (map (fun _ : EventType => Failure) l) =R= Failure.
 Proof.
@@ -828,99 +794,53 @@ induction l;intros. simpl. reflexivity.
 simpl. rewrite IHl. autorewrite with eqDB. reflexivity.
 Qed.
 
-Lemma Σ_list_prod_aux : forall l1 a c1 c2,
-Event a _;_ (a \ c1 _*_ Σ (map (fun a0 : EventType => Event a0 _;_ a0 \ c2) l1)) =R=
-Σ (map (fun a0 : EventType * EventType => Event (fst a0) _;_ (fst a0 \ c1 _*_ Event (snd a0) _;_ snd a0 \ c2)) (map (fun y : EventType => (a, y)) l1)).
-Proof.
-induction l1;intros;simpl.
-- auto_rwd_eqDB.
-- rewrite map_map. simpl. 
-  auto_rwd_eqDB. apply c_plus_ctx;auto with eqDB.
-  rewrite IHl1. rewrite map_map. simpl. reflexivity.
-Qed.
-
-
-Lemma Σ_list_prod : forall l0 l1 c1 c2,
-Σ (map (fun a => Event a _;_ (a \ c1 _*_ Σ (map (fun a0 : EventType => Event a0 _;_ a0 \ c2) l1))) l0) =R=
-Σ (map (fun a : EventType * EventType => Event (fst a) _;_ (fst a \ c1 _*_ Event (snd a) _;_ snd a \ c2)) (list_prod l0 l1)).
-Proof.
-induction l0;intros;simpl.
-- reflexivity.
-- rewrite map_app. rewrite Σ_app. rewrite IHl0. apply c_plus_ctx;auto with eqDB.
-  apply Σ_list_prod_aux.
-Qed.
-
-
-
-
-Lemma ΣΣ_prod : forall l0 l1 (P : EventType * EventType -> Contract), 
-Σ (map (fun a  => P a) (list_prod l0 l1))  =R=
-Σ (map (fun a0 => Σ (map (fun a1 => P (a0,a1)) l1)) l0).
-Proof.
-induction l0;intros.
-- simpl. reflexivity.
-- simpl. rewrite map_app. rewrite Σ_app.
-  eq_m_left. rewrite map_map. reflexivity.
-Qed. 
-(*
-
-Lemma Σ_plus_decompose
-Σ (map (fun a0 : EventType => P (a, a0) _+_ Σ (map (fun a1 : EventType => P (a1, a0)) l0)) l1)
-*)
-Lemma ΣΣ_prod_swap : forall l0 l1 (P : EventType * EventType -> Contract), 
-Σ (map (fun a0 => Σ (map (fun a1 => P (a0,a1)) l1)) l0)=R=
-Σ (map (fun a0 => Σ (map (fun a1 => P (a1,a0)) l0)) l1).
-Proof.
-induction l0;intros.
-- simpl. induction l1;intros;simpl;auto with eqDB. rewrite IHl1.
-  auto with eqDB.
-- simpl. rewrite Σ_decompose_fun. eq_m_left.
-Qed.
+Hint Resolve fold_Failure : eqDB.
 
 
 
 Ltac rwd_in_map f := rewrite map_ext_in_R ; try instantiate (1:=f);intros; auto_rwd_eqDB.
 
-Lemma derive_unfold : forall c, o c _+_ Σ (map (fun a : EventType => Event a _;_ a \ c) alphabet) =R= c.
+Lemma derive_unfold_seq : forall c1 c2, 
+o c1 _+_ Σ (map (fun a : EventType => Event a _;_ a \ c1) alphabet) =R= c1 ->
+o c2 _+_ Σ (map (fun a : EventType => Event a _;_ a \ c2) alphabet) =R= c2 -> 
+o (c1 _;_ c2) _+_ 
+Σ (map (fun a : EventType => Event a _;_ a \ (c1 _;_ c2)) alphabet) =R=
+c1 _;_ c2.
 Proof.
-induction c;intros;simpl in *;auto_rwd_eqDB.
-- rwd_in_map (fun (_ : EventType) => Failure).
-  induction alphabet. simpl. auto_rwd_eqDB.
-  simpl. rewrite IHl. auto_rwd_eqDB. 
-- auto_rwd_eqDB. rwd_in_map (fun a => Event e _;_ (if EventType_eq_dec e a then Success else Failure)).
-  * rewrite Σ_event. rewrite Σ_alphabet. auto_rwd_eqDB.
-  * intros. eq_event_destruct;subst. reflexivity.
-    auto_rwd_eqDB.
-- rwd_in_map (fun a => Event a _;_ a \ c1  _+_  Event a _;_ a \ c2);
-  intros; auto_rwd_eqDB.  rewrite Σ_decompose_fun. 
-  rewrite <- c_plus_assoc. rewrite (c_plus_comm (o _)).
-rewrite (c_plus_assoc (o _)).
-  rewrite IHc1. rewrite (c_plus_comm _ c1).
-  rewrite c_plus_assoc. rewrite IHc2. auto_rwd_eqDB.
+intros;simpl;auto_rwd_eqDB.
 - destruct (nu c1) eqn:Heqn.
   * rwd_in_map (fun a => Event a _;_ a \ c1 _;_ c2  _+_  Event a _;_ a \ c2);
-    intros; auto_rwd_eqDB.  rewrite Σ_decompose_fun.
-    rewrite Σ_decompose_Seq. rewrite <- IHc1 at 2.
-    rewrite <- IHc2 at 2. rewrite <- IHc2 at 3. auto_rwd_eqDB. eq_m_left.
+    intros; auto_rwd_eqDB.  rewrite Σ_split_plus.
+    rewrite Σ_factor_seq_r. rewrite <- H at 2.
+    rewrite <- H0 at 2. rewrite <- H0 at 3. auto_rwd_eqDB. eq_m_left.
     apply o_true in Heqn. rewrite Heqn.
     auto_rwd_eqDB. rewrite (c_plus_comm (Σ _ _;_ Σ _ )).
     eq_m_right. 
   * apply o_false in Heqn. rewrite Heqn in*. autorewrite with eqDB in *.
     rwd_in_map (fun a => Event a _;_ a \ c1 _;_ c2);
-    intros; auto_rwd_eqDB. rewrite Σ_decompose_Seq. 
-    rewrite IHc1. reflexivity.
-- auto_rwd_eqDB.
-  rewrite (map_ext_in_R _ (fun a : EventType =>  ((Event a _;_ (a \ c1 _*_ o c2) _+_ Event a _;_ ( a \ c1 _*_Σ (map (fun a : EventType => Event a _;_ a \ c2) alphabet))) 
+    intros; auto_rwd_eqDB. rewrite Σ_factor_seq_r. 
+    rewrite H. reflexivity.
+Qed.
+
+
+Lemma derive_unfold_par : forall c1 c2, 
+o c1 _+_ Σ (map (fun a : EventType => Event a _;_ a \ c1) alphabet) =R= c1 ->
+o c2 _+_ Σ (map (fun a : EventType => Event a _;_ a \ c2) alphabet) =R= c2 -> 
+o (c1 _*_ c2) _+_ 
+Σ (map (fun a : EventType => Event a _;_ a \ (c1 _*_ c2)) alphabet) =R=
+c1 _*_ c2.
+Proof.
+intros;simpl;auto_rwd_eqDB.
+rewrite (map_ext_in_R _ (fun a : EventType =>  ((Event a _;_ (a \ c1 _*_ o c2) _+_ Event a _;_ ( a \ c1 _*_Σ (map (fun a : EventType => Event a _;_ a \ c2) alphabet))) 
 _+_ (Event a _;_ (o c1 _*_ a \ c2) _+_ Event a _;_ (Σ (map (fun a : EventType => Event a _;_ a \ c1) alphabet) _*_ a \ c2 )))));
 
-  try solve [intros; rewrite <- c_distr_l; rewrite <- c_par_distr_l;  rewrite IHc2;
-  rewrite <- c_distr_l; rewrite <- c_distr_l;
-  rewrite <- c_par_distr_r; rewrite IHc1; reflexivity].
-  rewrite <- IHc1 at 2.
-  rewrite <- IHc2 at 2.
+try solve [intros; rewrite <- c_distr_l; rewrite <- c_par_distr_l;  rewrite H0;
+           rewrite <- c_distr_l; rewrite <- c_distr_l;
+           rewrite <- c_par_distr_r; rewrite H; reflexivity].
+rewrite <- H at 2. rewrite <- H0 at 2.
   auto_rwd_eqDB. repeat rewrite (c_par_comm (_ _+_ _)). auto_rwd_eqDB.
   rewrite c_plus_assoc. eq_m_left. 
-repeat rewrite Σ_decompose_fun.
+repeat rewrite Σ_split_plus.
 repeat rewrite <- c_plus_assoc. 
 remember (Σ (map (fun a : EventType => Event a _;_ (a \ c1 _*_ Σ (map (fun a0 : EventType => Event a0 _;_ a0 \ c2) alphabet))) alphabet)) as a.
 remember (Σ (map (fun a0 : EventType => Event a0 _;_ (Σ (map (fun a1 : EventType => Event a1 _;_ a1 \ c1) alphabet) _*_ a0 \ c2)) alphabet)) as b.
@@ -929,566 +849,141 @@ repeat rewrite <- c_plus_assoc.
 rewrite (c_plus_assoc _ b).
 apply c_plus_ctx.
   * rewrite c_plus_comm. apply c_plus_ctx.
-    ** destruct (o_destruct c1).
-      *** rewrite H. auto_rwd_eqDB. apply map_ext_in_R;
+    ** destruct (o_destruct c1);rewrite H1.
+      *** auto_rwd_eqDB. apply map_ext_in_R;
           intros; auto_rwd_eqDB.
-      *** rewrite H. auto_rwd_eqDB. 
+      *** auto_rwd_eqDB. 
           rewrite (map_ext_in_R _ (fun _ : EventType => Failure)).
           apply fold_Failure. intros. auto_rwd_eqDB.
-    ** destruct (o_destruct c2).
-      *** rewrite H. auto_rwd_eqDB. apply map_ext_in_R.
+    ** destruct (o_destruct c2);rewrite H1.
+      *** auto_rwd_eqDB. apply map_ext_in_R.
           intros. auto_rwd_eqDB.
-      *** rewrite H. auto_rwd_eqDB. 
+      *** auto_rwd_eqDB. 
           rewrite (map_ext_in_R _ (fun _ : EventType => Failure)).
           apply fold_Failure. intros. auto_rwd_eqDB.
-  * subst. rewrite Σ_par_distr.
-rewrite (map_ext_in_R _ ((fun a : EventType * EventType =>  Event (fst a) _;_ (fst a \ c1 _*_ Event (snd a) _;_ snd a \ c2) _+_ 
-Event (snd a) _;_ (Event (fst a) _;_ fst a \ c1 _*_ snd a \ c2))));
-    intros; auto_rwd_eqDB. rewrite Σ_decompose_fun.
- rewrite c_plus_comm. repeat rewrite ΣΣ_prod;simpl. apply c_plus_ctx.
-    ** apply map_ext_in_R. intros. rewrite Σ_decompose_Seq_l.
-       rewrite <- Σ_par_distr_aux. reflexivity.
-    ** pose proof (ΣΣ_prod_swap alphabet alphabet
-(fun p => Event (snd p) _;_ (Event (fst p) _;_ (fst p) \ c1 _*_ (snd p) \ c2))).
-       simpl in H. rewrite H. apply map_ext_in_R.
-       intros. rewrite Σ_decompose_Seq_l. apply c_seq_ctx;auto with eqDB.
-       rewrite Σ_par_distr_aux_r. reflexivity.
+  * subst. symmetry. rewrite Σ_par_ΣΣ.
+rewrite (map_ext_in_R _ (fun a0 : EventType => Σ (map (fun a1 : EventType => Event a0 _;_ (a0 \ c1 _*_ Event a1 _;_ a1 \ c2)) alphabet)
+                                           _+_ Σ (map (fun a1 : EventType => Event a1 _;_ (Event a0 _;_ a0 \ c1 _*_ a1 \ c2)) alphabet)));
+    intros; auto_rwd_eqDB;
+    try solve [rewrite <- Σ_split_plus; apply map_ext_in_R;
+    intros; auto_rwd_eqDB].
+ rewrite Σ_split_plus. rewrite c_plus_comm. apply c_plus_ctx.
+    ** rewrite ΣΣ_prod_swap. apply map_ext_in_R.
+       intros. rewrite Σ_factor_seq_l. apply c_seq_ctx;auto with eqDB.
+       rewrite Σ_factor_par_r. reflexivity.
+    ** apply map_ext_in_R. intros. 
+       rewrite Σ_factor_seq_l. apply c_seq_ctx;auto with eqDB.
+       rewrite Σ_factor_par_l. reflexivity.
 Qed.
 
-(*
-Lemma derive_unfold : forall c, (if nu c then Success else Failure) _+_ Σ (map (fun a : EventType => Event a _;_ a \ c) alphabet) =R= c.
+
+Lemma derive_unfold : forall c, o c _+_ Σ (map (fun a : EventType => Event a _;_ a \ c) alphabet) =R= c.
 Proof.
-induction c;intros;simpl in *.
-- rewrite (map_ext_in_R _ (fun _ => Failure)).
-  induction alphabet. simpl. auto_rwd_eqDB.
-  simpl. rewrite <- c_plus_assoc. rewrite (c_plus_comm Success).
-  rewrite c_plus_assoc.
-  rewrite IHl. auto_rwd_eqDB.
-  intros. destruct a;simpl; auto_rwd_eqDB.
-- rewrite (map_ext_in_R _ (fun _ => Failure)).
-  induction alphabet. simpl. auto_rwd_eqDB.
-  simpl. rewrite <- c_plus_assoc.
-  rewrite c_plus_idemp. apply IHl. 
-  intros. destruct a;simpl; auto_rwd_eqDB.
-- auto_rwd_eqDB. 
- rewrite (map_ext_in_R _ (fun a => Event e _;_ (if EventType_eq_dec e a then Success else Failure))).
-  * rewrite Σ_event. rewrite Σ_alphabet. auto_rwd_eqDB.
-  * intros. eq_event_destruct;subst. reflexivity.
-    auto_rwd_eqDB.
-- rewrite (map_ext_in_R _ (fun a => Event a _;_ a \ c1  _+_  Event a _;_ a \ c2));
-  intros; auto_rwd_eqDB.  rewrite Σ_decompose_fun.
-  destruct (nu c1);simpl.
-  * destruct (nu c2);simpl.
-    ** rewrite <- (c_plus_idemp Success).
-       rewrite c_plus_assoc. rewrite <- (c_plus_assoc _ (Σ _)).
-       rewrite IHc1. rewrite (c_plus_comm c1). rewrite <- c_plus_assoc.
-       rewrite IHc2. auto_rwd_eqDB.
-    ** autorewrite with eqDB in IHc2. rewrite IHc2.
-       rewrite <- c_plus_assoc. rewrite IHc1. reflexivity.
-  * destruct (nu c2);simpl.
-    ** autorewrite with eqDB in IHc1. rewrite IHc1.
-       rewrite (c_plus_comm c1). rewrite <- c_plus_assoc.  rewrite IHc2.
-       auto_rwd_eqDB. 
-    ** autorewrite with eqDB in *. rewrite IHc1. rewrite IHc2. reflexivity.
-- destruct (nu c1 && nu c2) eqn:Heqn.
-  * apply andb_prop in Heqn. destruct Heqn. rewrite H in*.
-    rewrite H0 in *.
-    rewrite (map_ext_in_R _ (fun a => Event a _;_ a \ c1 _;_ c2  _+_  Event a _;_ a \ c2));
-    intros; auto_rwd_eqDB.  rewrite Σ_decompose_fun.
-    rewrite Σ_decompose_Seq. rewrite <- IHc1.
-    rewrite <- IHc2. rewrite (c_distr_l (Success _+_ _)).
-    repeat rewrite (c_distr_r). auto_rwd_eqDB.
-    rewrite (c_plus_assoc Success). apply c_plus_ctx;auto with eqDB.
-    rewrite c_plus_assoc. apply c_plus_ctx;auto with eqDB.
-  * rewrite andb_false_iff in Heqn. destruct Heqn.
-    ** rewrite H in*. rewrite (map_ext_in_R _ (fun a => Event a _;_ a \ c1 _;_ c2));
-       intros; auto_rwd_eqDB. rewrite Σ_decompose_Seq. 
-          autorewrite with eqDB in IHc1. rewrite IHc1. reflexivity.
-    ** rewrite H in*. destruct (nu c1) eqn:Heqn.
-      *** rewrite (map_ext_in_R _ (fun a => Event a _;_ a \ c1 _;_ c2  _+_  Event a _;_ a \ c2));
-          intros; auto_rwd_eqDB.  rewrite Σ_decompose_fun.
-          rewrite Σ_decompose_Seq. autorewrite with eqDB in IHc2.
-          rewrite <- IHc1. auto_rwd_eqDB.
-          rewrite <- IHc2. auto_rwd_eqDB.
-      *** rewrite (map_ext_in_R _ (fun a => Event a _;_ a \ c1 _;_ c2));
-          intros; auto_rwd_eqDB. rewrite Σ_decompose_Seq.
-          autorewrite with eqDB in IHc1. rewrite IHc1. reflexivity.
-- rewrite <- IHc1 at 2.
-  rewrite <- IHc2 at 2.
-  auto_rwd_eqDB. repeat rewrite (c_par_comm (_ _+_ _)). auto_rwd_eqDB.
-  rewrite c_plus_assoc. apply c_plus_ctx.
-  * destruct (nu c1); destruct (nu c2);simpl;auto_rwd_eqDB.
-  *
-  rewrite 
- destruct (nu c1 && nu c2) eqn:Heqn.
-  * apply andb_prop in Heqn. destruct Heqn.
- rewrite H in*. 
-    rewrite H0 in IHc2.
- Check c_par_event.
-    rewrite (map_ext_in_R _ (fun a => Event a _;_ (a \ c1 _*_ c2)  _+_  Event a _;_ (c1 _*_ a \ c2)));
-          intros; auto_rwd_eqDB.
- Check c_par_event. 
-rewrite Σ_decompose_fun.
- Check c_par_event.
-    rewrite <- IHc1.
-    rewrite <-  rewrite <- (c_par_comm c2). auto_rwd_eqDB.
-    rewrite <- IHc2. repeat rewrite (c_par_comm (_ _+_ _)).
-    auto_rwd_eqDB. rewrite Σ_par_distr. 
- Check c_par_event.*)
+induction c;intros.
+- simpl;auto_rwd_eqDB.
+- simpl;auto_rwd_eqDB. rwd_in_map (fun (_ : EventType) => Failure).
+- rwd_in_map (fun a => Event e _;_ (if EventType_eq_dec e a then Success else Failure)).
+  * rewrite Σ_factor_seq_l. rewrite Σ_alphabet. auto_rwd_eqDB.
+  * simpl. eq_event_destruct;subst; auto_rwd_eqDB.
+- simpl;auto_rwd_eqDB. rwd_in_map (fun a => Event a _;_ a \ c1  _+_  Event a _;_ a \ c2);
+  intros; auto_rwd_eqDB. rewrite Σ_split_plus. 
+  rewrite <- c_plus_assoc. rewrite (c_plus_comm (o _)).
+rewrite (c_plus_assoc (o _)).
+  rewrite IHc1. rewrite (c_plus_comm _ c1).
+  rewrite c_plus_assoc. rewrite IHc2. auto_rwd_eqDB.
+- auto using derive_unfold_seq.
+- auto using derive_unfold_par.
+Qed.
+
 
 Lemma plus_norm_c_eq : forall c, plus_norm c =R= c.
 Proof.
-intros. funelim (plus_norm c).
-stuck_tac.
+intros. funelim (plus_norm c). stuck_tac.
 - symmetry. auto using Stuck_eq_Failure.
-- destruct (nu c) eqn:Heqn.
-  * rewrite map_ext_in_R. 2: { intros. rewrite H at 1;auto. eapply c_refl. }
- 
-  * reflexivity.
-induction c;intros.
-4: { simp plus_norm. stuck_tac.
-  * inversion s.
-    apply Stuck_eq_Failure in H2. apply Stuck_eq_Failure in H3.
-    rewrite H2. rewrite H3. auto_rwd_eqDB.
-  * simpl. destruct (nu c1 || nu c2) eqn:Heqn.
-    **
-- auto_rwd_eqDB. 
-- auto_rwd_eqDB. 
+- rewrite map_ext_in_R. apply derive_unfold.
+  intros. rewrite H at 1;auto. eapply c_refl.
+Qed.
 
-Lemma plus_norm_c_eq : forall c, plus_norm c =R= c.
+
+(**********************Define Sigma normal form and show plus_norm always returns a Sigma normal form*************************************)
+Inductive Atom : Contract -> Prop :=
+| AFailure : Atom Failure
+| ASuccess : Atom Success.
+Hint Constructors Atom : eqDB.
+
+Lemma Atom_i_Sequential : forall c, Atom c -> Sequential c.
 Proof.
-induction c;intros.
-4: { simp plus_norm. stuck_tac.
-  * inversion s.
-    apply Stuck_eq_Failure in H2. apply Stuck_eq_Failure in H3.
-    rewrite H2. rewrite H3. auto_rwd_eqDB.
-  * simpl. destruct (nu c1 || nu c2) eqn:Heqn.
-    **
-- auto_rwd_eqDB. 
-- auto_rwd_eqDB. 
+intros. inversion H;auto with eqDB.
+Qed.
 
-- destruct (plus_norm_trans (Event e)).
-  eapply c_core;simpl;  eauto. symmetry. auto using trans_plus_norm_Event.
+Hint Resolve Atom_i_Sequential : eqDB.
 
+Inductive NormalForm : Contract -> Prop :=
+| NFA c (H: Atom c) : NormalForm c
+| NFList c es l (H: Atom c) (H1: forall a, In a l -> NormalForm a) : NormalForm (c _+_ Σ (map (fun x => Event (fst x) _;_ snd x) (combine es l))).
 
-  apply trans_plus_norm_Event in H.
-  pose proof (translate_aux_spec H). eapply NormalForm_trans. simp plus_norm. stuck_tac. symmetry. auto using Stuck_eq_Failure.
-  simpl. pose proof in_alphabet. induction alphabet. 
-  specialize H with Transfer. simpl in H. contradiction.
-   simpl. rewrite IHl. eq_event_destruct;subst.
-   auto_rwd_eqDB. auto_rwd_eqDB. rewrite e0 in e1. discriminate.
-  * auto_rwd_eqDB.
-
- apply Stuck_eq_Failure.  simp plus_norm. auto with eqDB.
-
-Section axiomatization.
-
-  Hypothesis sum_rule : forall c, exists c', NormalForm c' /\ c =R= c'.
-
-  Lemma c_eq_completeness : forall (c0 c1 : Contract),(forall s : Trace, s =~ c0 <-> s =~ c1) ->  c0 =R= c1.
-  Proof.
-  intros. destruct (sum_rule c0). destruct (sum_rule c1). destruct_ctx.
-  pose proof c_eq_soundness H3. setoid_rewrite H4 in H. 
-  pose proof c_eq_soundness H2. setoid_rewrite H5 in H.
-  rewrite H3. rewrite H2.
-  apply NormalForm_trans in H0. apply NormalForm_trans in H1. destruct_ctx. 
-  eapply c_core. eauto. eauto. apply CSLEQ.c_eq_completeness.
-  setoid_rewrite <- translate_aux_spec. eapply H. all: eauto.
-  Qed.
-
-End axiomatization.
- 
-
-
-
-
-
-
-Lemma plus_norm_sequential : forall (c : Contract), Sequential (plus_norm c).
-Proof. 
-intros. funelim (plus_norm c).
-destruct (stuck_dec c).
-- constructor.
-- destruct (nu c).
-  * constructor. constructor. induction alphabet.
-    ** simpl. constructor.
-    ** simpl. repeat constructor. auto. assumption.
-  * induction alphabet.
-    ** simpl. constructor.
-    ** simpl. repeat constructor. auto. assumption.
-Defined.
-
-
-
-(*
-Lemma stuck_c_eq_Failure : forall c c', translate_aux c = Some c' -> Stuck c -> CSLEQ.c_eq CSLC.Failure c'.
-Proof. Admitted.*)
-
-Ltac core_tac := eapply c_core;simpl;eauto with eqDB.
-
-Lemma stuck_c_eq_Failure : forall c, Stuck c -> Failure =R= c.
+Lemma Sequential_Σ : forall l, (forall c, In c l -> Sequential c) -> Sequential (Σ l).
 Proof.
-intros. induction H; try solve [core_tac].
-- rewrite <- IHStuck1. rewrite <- IHStuck2. core_tac.
-- rewrite <- IHStuck.
-
-Lemma plus_norm_eq : forall p, plus_norm p =R= p.
-Proof. 
-intros. funelim (plus_norm p). destruct (stuck_dec c).
-- induction s.
-  * eapply c_core;simpl;eauto with eqDB.
-  * destruct (translate_aux c) eqn:Heqn.
-  * apply stuck_c_eq_Failure in Heqn as H';auto. eapply c_core;simpl;eauto.
-  *
-    simpl. eauto. eapply Heqn. eauto.
-    simpl. inversion s.
+induction l;intros; auto with eqDB.
+simpl. constructor. auto using in_eq.
+apply IHl. intros. apply H. simpl. now right. 
+Qed.
 
 
-
-Theorem c_eq_complete : forall c0 c1, (forall s, s =~ c0 <-> s=~c1) -> c0 =R= c1.
+Lemma NormalForm_i_Sequential : forall c, NormalForm c -> Sequential c.
 Proof.
-intros. rewrite <- plus_norm_eq. rewrite <- (plus_norm_eq c1).
-destruct (correct_translation c0). destruct (correct_translation c1).
-destruct_ctx. unfold translate in *.
- eapply c_core;eauto. apply CSLEQ.c_eq_completeness. 
- setoid_rewrite <- H3. setoid_rewrite <- H2. auto.
+intros. induction H;auto with eqDB.
+- inversion H;
+  constructor; subst; auto with eqDB;
+  apply Sequential_Σ; intros;
+  rewrite in_map_iff in *; destruct_ctx; subst; try constructor;
+  (try constructor); destruct x; apply in_combine_r in H3; auto.
+Qed.
+
+Lemma NormalForm_trans : forall c, NormalForm c -> exists c', translate_aux c = Some c'.
+Proof.
+intros. apply translate_aux_sequential. auto using NormalForm_i_Sequential.
+Qed.
+
+Lemma decompose_map : 
+forall es c, map (fun e => Event e _;_ plus_norm (e \ c)) es = map (fun x => (Event (fst x) _;_ snd x)) (combine es (map (fun e => plus_norm (e \ c) ) es)).
+Proof.
+induction es;intros.
+- simpl. auto.
+- simpl. rewrite IHes. auto.
+Qed. 
+
+Lemma plus_norm_NormalForm : forall c, NormalForm (plus_norm c).
+Proof.
+intros. funelim (plus_norm c). stuck_tac.
+- constructor. constructor.
+- rewrite decompose_map. erewrite map_ext. eapply NFList.
+  * destruct (o_destruct c); rewrite H0; auto with eqDB.
+  * intros. rewrite in_map_iff in *. destruct_ctx.
+    subst. auto.
+  * intros. simpl. auto.
 Qed.
 
 
 
-
-
-
-
-
-
-
-
-
-
-Inductive NormalForm : list Contract -> Prop :=
-| NF_nil : NormalForm []
-| NF_cons e c l (H: NormalForm l) : NormalForm ((Event e _;_ c):: l).
-
-
-
-Equations interleavings  (s0 s1: Trace) : (list Trace) by  wf ((length s0) + (length s1)) :=
-interleavings [] s1 := [s1];
-interleavings s0 [] := [s0];
-interleavings (e0::s0') (e1::s1') := (map (fun s => e0::s) (interleavings s0' (e1::s1'))) ++ 
-                                     (map (fun s => e1::s) (interleavings (e0::s0') s1')).
-Next Obligation.  lia. Defined.
-
-Theorem interleavings_i_interleave_fun : forall (s0 s1 s : Trace), In s (interleavings s0 s1) -> interleave_fun s0 s1 s.
+Lemma sum_decomposition_exists : forall c, exists c', NormalForm c' /\ c =R= c'.
 Proof.
-intros. funelim (interleavings s0 s1).
-- simp interleavings in H. simpl in H. destruct H;try contradiction. subst. auto with cDB.
-- simp interleavings in H. simpl in H. destruct H;try contradiction. subst. auto with cDB.
-- simp interleavings in H1. apply in_app_or in H1. destruct H1.
-  * rewrite in_map_iff in H1. destruct_ctx. apply H in H2. 
-    subst. auto with cDB.
-  * rewrite in_map_iff in H1. destruct_ctx. apply H0 in H2. 
-    subst. auto with cDB.
-Qed.
-
-Lemma in_one : forall (A:Type) (a a0 : A), In a [a0] -> a = a0.
-Proof.
-intros. simpl in H. destruct H;try contradiction;auto.
-Qed.
-
-Lemma interleavings_nil_r : forall s, interleavings s []  = [s].
-Proof.
-induction s;intros; reflexivity.
-Qed.
-
-Lemma interleavings_one_l : forall (s : Trace)e,  In (e :: s) (interleavings [e] s).
-Proof.
-intros. funelim (interleavings [e] s).
--  simp interleavings. apply in_eq.
-- rewrite <- Heqcall. apply in_or_app. left. rewrite in_map_iff.
-  exists (e0::l0). split;auto. simp interleavings. apply in_eq.
-Qed.
-
-Lemma interleavings_one_r : forall (s : Trace)e,  In (e :: s) (interleavings s [e]).
-Proof.
-intros. funelim (interleavings s [e]).
--  simp interleavings. apply in_eq.
-- rewrite <- Heqcall. apply in_or_app. right. rewrite in_map_iff.
-  exists (e::l). split;auto. simp interleavings. apply in_eq.
-Qed.
-
-Lemma interleavings_extend_l : forall (s0 s1 s : Trace) e,  In s (interleavings s0 s1) ->
-In (e::s) (interleavings (e::s0) s1).
-Proof. 
-intros. destruct s1. simp interleavings in*. rewrite interleavings_nil_r in *. 
-apply in_one in H. subst. apply in_eq. 
-simp interleavings. apply in_or_app. left. rewrite in_map_iff.
-exists s. split;auto.
-Qed.
-
-Lemma interleavings_extend_r : forall (s0 s1 s : Trace) e,  In s (interleavings s0 s1) ->
-In (e::s) (interleavings s0 (e::s1)).
-Proof. 
-intros. destruct s0. simp interleavings in*. apply in_one in H. subst.
-apply in_eq. 
-simp interleavings. apply in_or_app. right. rewrite in_map_iff.
-exists s. split;auto.
-Qed.
-
-Theorem interleave_fun_i_interleavings : forall (s s0 s1: Trace), interleave_fun s0 s1 s
--> In s (interleavings s0 s1).
-Proof.
-induction s;intros. simpl in H. destruct H. subst. simpl. now left.
-simpl in H. destruct s0.
-- subst. simpl. now left.
-- destruct H.
-  * destruct H. subst. apply IHs in H0. auto using interleavings_extend_l.
-  * destruct s1.
-    ** simp interleavings. inversion H. apply in_eq.
-    ** destruct H. subst. apply IHs in H0. auto using interleavings_extend_r.
-Qed.
-
-Theorem interleave_fun_iff_interleavings : forall (s s0 s1: Trace),
-interleave_fun s0 s1 s <-> In s (interleavings s0 s1).
-Proof. split; auto using interleave_fun_i_interleavings, interleavings_i_interleave_fun.
+intros. exists (plus_norm c). split. apply plus_norm_NormalForm. symmetry. apply plus_norm_c_eq.
 Qed.
 
 
+(*************Completeness = rewrite to normal form + appeal to CSL_core ***********)
 
-Fixpoint L (c : Contract) : list Trace :=
-match c with
-| Success => [[]]
-| Failure => []
-| Event e => [[e]]
-| c0 _+_ c1 => (L c0) ++ (L c1)
-| c0 _;_ c1 => map (fun p => (fst p)++(snd p)) (list_prod (L c0) (L c1))
-| c0 _*_ c1 => flat_map (fun p => interleavings (fst p) (snd p)) (list_prod (L c0) (L c1))
-end.
-
-
-Lemma Matches_member : forall (s : Trace)(c : Contract), s =~ c -> In s (L c). 
+Lemma c_eq_completeness : forall (c0 c1 : Contract),(forall s : Trace, s =~ c0 <-> s =~ c1) ->  c0 =R= c1.
 Proof.
-intros. induction H ; simpl ; try solve [auto using in_or_app || auto using in_or_app ].
-- rewrite in_map_iff. exists (s1,s2). rewrite in_prod_iff. split;auto.
-- rewrite in_flat_map. exists (s1,s2). split.
-  * rewrite in_prod_iff. split;auto.
-  * simpl. rewrite <- interleave_fun_iff_interleavings. 
-    now rewrite <- interl_iff_fun.
+intros. destruct (sum_decomposition_exists c0). destruct (sum_decomposition_exists c1). destruct_ctx.
+pose proof c_eq_soundness H3. setoid_rewrite H4 in H. 
+pose proof c_eq_soundness H2. setoid_rewrite H5 in H.
+rewrite H3. rewrite H2.
+apply NormalForm_trans in H0. apply NormalForm_trans in H1. destruct_ctx. 
+eapply c_core. eauto. eauto. apply CSLEQ.c_eq_completeness.
+setoid_rewrite <- translate_aux_spec. eapply H. all: eauto.
 Qed.
-
-Lemma member_Matches : forall (c : Contract)(s : Trace), In s (L c) -> s =~ c. 
-Proof.
-induction c;intros;simpl in*; try solve [ destruct H;try contradiction; subst; constructor].
-- apply in_app_or in H. destruct H; auto with cDB.
-- rewrite in_map_iff in H. destruct_ctx. destruct x.
-  rewrite in_prod_iff in H0. destruct H0. simpl in H.
-  subst. auto with cDB.
-- rewrite in_flat_map in H. destruct_ctx.
-  rewrite <- interleave_fun_iff_interleavings in H0. 
-  destruct x. rewrite in_prod_iff in H. destruct H.
-  simpl in*. rewrite <- interl_iff_fun in H0. eauto with cDB.
-Qed.
-
-Theorem Matches_iff_member : forall s c, s =~ c <-> In s (L c).
-Proof.
-split; auto using Matches_member,member_Matches.
-Qed.
-
-Lemma Matches_incl : forall (c0 c1 : Contract), (forall (s : Trace), s =~ c0 -> s =~ c1) -> 
-incl (L c0) (L c1).
-Proof.
-intros. unfold incl. intros. rewrite <- Matches_iff_member in *. auto.
-Qed.
-
-Lemma comc_equiv_destruct : forall (c0 c1: Contract),(forall s : Trace, s =~ c0 <-> s =~ c1) <->
-(forall s : Trace, s =~ c0 -> s =~ c1) /\ (forall s : Trace, s =~ c1 -> s =~ c0).
-Proof.
- split ; intros.
-- split;intros; specialize H with s; destruct H; auto.
-- destruct H. split;intros;auto.
-Qed.
-
-
-Theorem Matches_eq_i_incl_and : forall (c0 c1 : Contract), (forall (s : Trace), s =~ c0 <-> s =~ c1) -> 
-incl (L c0) (L c1) /\ incl (L c1) (L c0) .
-Proof.
-intros. apply comc_equiv_destruct in H. destruct H. split; auto using Matches_incl. 
-Qed.
-
-
-
-
-Fixpoint Π (s : Trace) :=
-match s with
-| [] => Success
-| e::s' => (Event e) _;_ (Π s')
-end.
-
-Lemma Π_app : forall (l1 l2 : Trace), Π l1 _;_ Π l2 =R= Π (l1++l2).
-Proof.
-induction l1;intros;simpl; auto_rwd_eqDB.
-rewrite <- IHl1. auto_rwd_eqDB.
-Qed.
-
-(*
-Definition Π (l : list Trace) := Σ (map Π l).
-Hint Unfold Π : eqDB.*)
-
-
-Lemma Π_distr_aux : forall (ss : list Trace) (s : Trace), Π s _;_ (Σ (map Π ss)) =R=
- Σ (map (fun x => Π (fst x ++ snd x)) (map (fun y : list EventType => (s, y)) ss)).
-Proof.
-induction ss;intros;simpl;auto_rwd_eqDB.
-apply c_plus_ctx;auto using Π_app.
-Qed.
-
-Lemma Π_distr_aux2 : forall c l0, c _;_ Σ (map Π l0) =R=
- Σ (map (fun x => c _;_ Π x) l0).
-Proof.
-induction l0;intros;simpl;auto_rwd_eqDB.
-Qed.
-
-
-(*
-Lemma Π_distr2 : forall l0 l1,  Σ l0 _;_ Σ l1 =R=
- Σ (map (fun x => (fst x) _;_ (snd x)) (list_prod l0 l1)).
-Proof.
-induction l0;intros;simpl. auto_rwd_eqDB.
-repeat rewrite map_app. rewrite Σ_app. rewrite <- IHl0.
-auto_rwd_eqDB. rewrite map_map. simpl. 
-apply c_plus_ctx; auto using Π_distr_aux2 with eqDB. 
-Qed.*)
-
-(*Mention in report*)
-
-
-Lemma exchange : forall p q r s, 
- (p _*_ q) _;_ (r _*_ s) _+_ (p _;_ r) _*_ (q _;_ s) =R= (p _;_ r) _*_ (q _;_ s).
-Proof. Admitted.
-
-Lemma exchange2 : forall a b c, 
- a _*_ (b _;_ c) _+_ (a _*_ b) _;_ c =R=
- a _*_ (b _;_ c).
-Proof. Admitted.
-
-
-(*
-Lemma Π_par_aux2 : forall (s0 s1 : Trace) e, Event e _;_ Π s0 _*_ Π s1 =R=
- Σ (map (fun x => Π (e::x)) (interleavings s0 s1)).
-Proof.
-intros. simpl. rewrite <- Π_distr_aux2. 
-apply c_seq_ctx. auto with eqDB.*)
-
-Lemma Σ_interleavings : forall (s0 s1 : Trace),
-Σ (map Π (interleavings s0 s1)) =R= (Π s0) _*_ (Π s1).
-Proof.
-intros. funelim (interleavings s0 s1).
-- simp interleavings. simpl. rewrite c_par_comm. auto_rwd_eqDB.
-- rewrite interleavings_nil_r. simpl. auto_rwd_eqDB.
-- simp interleavings. rewrite map_app. rewrite Σ_app.
-  repeat rewrite map_map. clear Heqcall. simpl.
-  repeat rewrite <- Π_distr_aux2. rewrite H.
-  rewrite H0. simpl.
-
-  remember ( Π l) as c. remember (Π l0) as d.
-  now rewrite c_par_event.
-Qed.
-
-
-Lemma Π_distr : forall l0 l1,  Σ (map Π l0) _;_ Σ (map Π l1) =R=
- Σ (map (fun x => Π (fst x ++ snd x)) (list_prod l0 l1)).
-Proof.
-induction l0;intros;simpl. auto_rwd_eqDB.
-repeat rewrite map_app. rewrite Σ_app. rewrite <- IHl0.
-auto_rwd_eqDB. 
-apply c_plus_ctx; auto using Π_distr_aux with eqDB. 
-Qed.
-
-(*
-
-
-Lemma Σ_interleavings_aux : forall (s0 s1 : Trace) c,
-Σ (map (fun x => c _;_ Π x) (interleavings s0 s1)) =R= c _;_ ((Π s0) _*_ (Π s1)).
-Proof.
-intros. funelim (interleavings s0 s1).
-- simp interleavings. simpl. rewrite c_par_comm. auto_rwd_eqDB.
-- rewrite interleavings_nil_r. simpl. auto_rwd_eqDB.
-- simp interleavings. rewrite map_app.
-  rewrite Σ_app. rewrite map_map.
-  rewrite map_ext_in_R.
-  * rewrite H. rewrite map_map. simpl. rewrite map_ext_in_R.
-    ** rewrite H0. simpl.
-  setoid_rewrite <- c_seq_assoc. rewrite H0.
-
- rewrite <- c_seq_neut. rewrite <- exchange. rewrite <- par_der. reflexivity. auto with eqDB. apply par_der.  rewrite simpl in H0. rewrite 
-  rewrite map_map. simpl.
-  rewrite <- H.
-*)
-
-
-
-Lemma Π_par_aux : forall (ss : list Trace) (s : Trace), Π s _*_ (Σ (map Π ss)) =R=
- Σ (map Π (flat_map (fun x => interleavings (fst x) (snd x)) (map (fun y : list EventType => (s, y)) ss))).
-Proof.
-induction ss;intros;simpl;auto_rwd_eqDB.
-rewrite map_app. rewrite Σ_app. rewrite <- IHss.
-rewrite c_par_distr_l. rewrite Σ_interleavings. auto with eqDB.
-Qed.
-
-
-Lemma Π_distr_par : forall l0 l1,  Σ (map Π l0) _*_ Σ (map Π l1) =R=
- Σ (map Π (flat_map (fun x =>(interleavings (fst x) (snd x))) (list_prod l0 l1))).
-Proof.
-induction l0;intros;simpl. rewrite c_par_comm. auto_rwd_eqDB.
-rewrite flat_map_app. rewrite map_app. rewrite  Σ_app.
-rewrite <- IHl0. rewrite <- Π_par_aux. 
-rewrite c_par_comm. rewrite c_par_distr_l.
- auto with eqDB. 
-Qed.
-
-
-
-Theorem Π_L_ceq : forall (c : Contract), Σ (map Π (L c)) =R= c.
-Proof.
-induction c; simpl; try solve [auto_rwd_eqDB].
-- rewrite map_app. rewrite Σ_app.
-  auto using c_plus_ctx. 
-- rewrite map_map.
-  rewrite <- IHc1 at 2. rewrite <- IHc2 at 2.
-  symmetry. apply Π_distr.
-- rewrite <- IHc1 at 2. rewrite <- IHc2 at 2.
-  rewrite Π_distr_par. auto with eqDB.
-Qed.
-
-
-
-Lemma c_eq_completeness : forall (c0 c1 : Contract), (forall s : Trace, s =~ c0 <-> s =~ c1) -> c0 =R= c1.
-Proof.
-intros. rewrite <- Π_L_ceq. rewrite <- (Π_L_ceq c1). 
-apply Matches_eq_i_incl_and in H.
-destruct H. auto using incl_map, incl_Σ_c_eq.
-Qed.
-
-
-
-Theorem Matches_iff_c_eq : forall c0 c1, (forall s, s =~ c0 <-> s =~ c1) <-> c0 =R= c1.
-Proof.
-split; auto using c_eq_completeness, c_eq_soundness.
-Qed.
-
-Lemma L_Σ : forall l, L (Σ l) = flat_map L l.
-Proof.
-induction l;intros;simpl;auto. now rewrite IHl.
-Qed.
-
-
-
-
-
-
-
-
-
 
 
 
